\documentclass[../notes.tex]{subfiles}

\begin{document}

% !TEX root = ../notes.tex

\subsection{Units and Counits Speed-run}
We quickly recall that the transpose of $f:Fc\to d$ is $Gf\circ\eta_c$, and the transpose of $g:c\to Gd$ is $\varepsilon_d\circ Fg$.

We now continue the proof from last class.
\adjointbyunits*
\begin{proof}
	Suppose that we have functors $F:\mc C\rightleftharpoons\mc D:G$ with $\eta$ and $\varepsilon$ satisfying the needed triangle equations.

	We now define our adjunction by hand. Namely, we define
	\[\varphi:\op{Mor}_\mc D(Fc,d)\to\op{Mor}_\mf C(c,Gd)\]
	by sending $f$ to $Gf\circ\eta_c$ by hand. Similarly, we define
	\[\psi:\op{Mor}_\mc C(c,Gd)\to\op{Mor}_\mc D(Gc,d)\]
	by $\psi:g\mapsto\varepsilon_d\circ Fg$. To check that these are inverses, we see that
	\[\psi\varphi(f)=\psi(Gf\circ\eta_c)=\varepsilon_d\circ FGf\circ F\eta_c.\]
	Computing, we push $\varepsilon_d$ through via the following triangle.
	% https://q.uiver.app/?q=WzAsNCxbMCwwLCJGR0ZjIl0sWzEsMCwiRkdkIl0sWzEsMSwiZCJdLFswLDEsIkZjIl0sWzAsMSwiRkdmIl0sWzEsMiwiXFx2YXJlcHNpbG9uX2QiXSxbMCwzLCJcXHZhcmVwc2lsb25fe0ZjfSIsMl0sWzMsMiwiZiIsMl1d
	\[\begin{tikzcd}
		FGFc & FGd \\
		Fc & d
		\arrow["FGf", from=1-1, to=1-2]
		\arrow["{\varepsilon_d}", from=1-2, to=2-2]
		\arrow["{\varepsilon_{Fc}}"', from=1-1, to=2-1]
		\arrow["f"', from=2-1, to=2-2]
	\end{tikzcd}\]
	This commutes by naturality. As such, we find that
	\[\psi\varphi(f)=f\circ\varepsilon_{Fc}\circ F\eta_c=f,\]
	where in the last equality we have used the triangle equations.

	For the other inverse, we compute
	\[\varphi\psi(g)=\varphi(\varepsilon_d\circ Fg)=G\varepsilon_d\circ GFGg\circ\eta_c.\]
	As such, we draw the following naturality square to push out $\eta$.
	% https://q.uiver.app/?q=WzAsNCxbMCwwLCJjIl0sWzEsMCwiR2QiXSxbMSwxLCJHRkdkIl0sWzAsMSwiR0ZjIl0sWzEsMiwiXFxldGFfe0dkfSJdLFswLDMsIlxcZXRhX2MiLDJdLFswLDEsImciXSxbMywyLCJHRmciLDJdXQ==
	\[\begin{tikzcd}
		c & Gd \\
		GFc & GFGd
		\arrow["{\eta_{Gd}}", from=1-2, to=2-2]
		\arrow["{\eta_c}"', from=1-1, to=2-1]
		\arrow["g", from=1-1, to=1-2]
		\arrow["GFg"', from=2-1, to=2-2]
	\end{tikzcd}\]
	Thus, we compute
	\[\varphi\psi(g)=G\varepsilon_d\circ\eta_{Gd}\circ g=g,\]
	where we once again finished by the triangle equations.

	It remains to check naturality. We use \autoref{lem:betteradjoint}, of which we show the other direction. Namely, we show that the left square below makes the right square commutes.
	\[\begin{tikzcd}[ampersand replacement=\&]
		Fc \& d \& c \& Gd \\
		{Fc'} \& {d'} \& {c'} \& {Gd'}
		\arrow["{f}", from=1-1, to=1-2]
		\arrow["{g}"', from=2-1, to=2-2]
		\arrow["Fh"', from=1-1, to=2-1]
		\arrow["k", from=1-2, to=2-2]
		\arrow["h"', from=1-3, to=2-3]
		\arrow["{\varphi f}", from=1-3, to=1-4]
		\arrow["{\varphi g}"', from=2-3, to=2-4]
		\arrow["Gk", from=1-4, to=2-4]
	\end{tikzcd}\]
	The left square commuting gives $kf=gFf$, so
	\[Gk\circ Gg\circ\eta_c=Gg\circ GFh\circ\eta_c\tag{$*$}\label{eq:startingwhatever}\]
	by throwing through $G$ and putting $\eta_c$ on the right. The left-hand side is now $Gk\circ\varphi(f)$. On the other side, we draw the following naturality square.
	% https://q.uiver.app/?q=WzAsNCxbMCwwLCJjIl0sWzEsMCwiR0ZjIl0sWzAsMSwiYyciXSxbMSwxLCJHRmMnIl0sWzAsMiwiaCIsMl0sWzEsMywiR0ZoIl0sWzAsMSwiXFxldGFfYyJdLFsyLDMsIlxcZXRhX3tjJ30iLDJdXQ==
	\[\begin{tikzcd}
		c & GFc \\
		{c'} & {GFc'}
		\arrow["h"', from=1-1, to=2-1]
		\arrow["GFh", from=1-2, to=2-2]
		\arrow["{\eta_c}", from=1-1, to=1-2]
		\arrow["{\eta_{c'}}"', from=2-1, to=2-2]
	\end{tikzcd}\]
	As such, our right-hand side of \autoref{eq:startingwhatever} becomes
	\[Gk\circ\varphi(f)=\varphi(g)\circ h,\]
	which gives the commutativity of the desired square.
\end{proof}

\subsection{Morphism of Adjunctions}
We now begin discussion. We start with the following definition.
\begin{definition}[Morphism of adjunctions]
	A \textit{morphism of adjunctions} from $F\adjoint G$ to $F'\adjoint G'$ is a pair of functors $H:\mc C\to\mc C'$ and $K:\mc D\to mc D'$ so that the following two diagrams commute.
	% https://q.uiver.app/?q=WzAsOCxbMCwwLCJcXG1jIEMiXSxbMSwwLCJcXG1jIEMnIl0sWzAsMSwiXFxtYyBEIl0sWzEsMSwiXFxtYyBEJyJdLFsyLDAsIlxcbWMgQyJdLFszLDAsIlxcbWMgQyciXSxbMiwxLCJcXG1jIEQiXSxbMywxLCJcXG1jIEQnIl0sWzAsMiwiRiIsMl0sWzAsMSwiSCJdLFsxLDMsIkYnIl0sWzIsMywiSyIsMl0sWzQsNSwiSCJdLFs2LDQsIkciXSxbNyw1LCJHJyIsMl0sWzYsNywiSyIsMl1d&macro_url=https%3A%2F%2Fraw.githubusercontent.com%2FdFoiler%2Fnotes%2Fmaster%2Fnir.tex
	\[\begin{tikzcd}
		{\mc C} & {\mc C'} & {\mc C} & {\mc C'} \\
		{\mc D} & {\mc D'} & {\mc D} & {\mc D'}
		\arrow["F"', from=1-1, to=2-1]
		\arrow["H", from=1-1, to=1-2]
		\arrow["{F'}", from=1-2, to=2-2]
		\arrow["K"', from=2-1, to=2-2]
		\arrow["H", from=1-3, to=1-4]
		\arrow["G", from=2-3, to=1-3]
		\arrow["{G'}"', from=2-4, to=1-4]
		\arrow["K"', from=2-3, to=2-4]
	\end{tikzcd}\]
	Additionally, we require one of the following (equivalent) conditions.
	\begin{listalph}
		\item $H\eta=\eta'H$.
		\item $K\varepsilon=\varepsilon'K$.
		\item The following diagram commutes.
		% https://q.uiver.app/?q=WzAsNixbMCwwLCJcXG9we01vcn1fXFxtYyBEKEZjLGQpIl0sWzEsMCwiXFxvcHtNb3J9X3tcXG1jIEN9KGMsR2QpIl0sWzAsMSwiXFxvcHtNb3J9X3tcXG1jIEQnfShLRmMsS2QpIl0sWzAsMiwiXFxvcHtNb3J9X3tcXG1jIEQnfShGJ0hjLEtkKSJdLFsxLDIsIlxcb3B7TW9yfV97XFxtYyBDJ30oSGMsRydLZCkiXSxbMSwxLCJcXG9we01vcn1fe1xcbWMgQyd9KEhjLEhHZCkiXSxbMCwyLCJLIiwyXSxbMiwzLCIiLDIseyJsZXZlbCI6Miwic3R5bGUiOnsiaGVhZCI6eyJuYW1lIjoibm9uZSJ9fX1dLFsxLDUsIkgiXSxbMCwxXSxbMyw0XSxbNSw0LCIiLDAseyJsZXZlbCI6Miwic3R5bGUiOnsiaGVhZCI6eyJuYW1lIjoibm9uZSJ9fX1dXQ==&macro_url=https%3A%2F%2Fraw.githubusercontent.com%2FdFoiler%2Fnotes%2Fmaster%2Fnir.tex
		\[\begin{tikzcd}
			{\op{Mor}_\mc D(Fc,d)} & {\op{Mor}_{\mc C}(c,Gd)} \\
			{\op{Mor}_{\mc D'}(KFc,Kd)} & {\op{Mor}_{\mc C'}(Hc,HGd)} \\
			{\op{Mor}_{\mc D'}(F'Hc,Kd)} & {\op{Mor}_{\mc C'}(Hc,G'Kd)}
			\arrow["K"', from=1-1, to=2-1]
			\arrow[Rightarrow, no head, from=2-1, to=3-1]
			\arrow["H", from=1-2, to=2-2]
			\arrow[from=1-1, to=1-2]
			\arrow[from=3-1, to=3-2]
			\arrow[Rightarrow, no head, from=2-2, to=3-2]
		\end{tikzcd}\]
	\end{listalph}
	Here, $\varepsilon,\eta$ are the unit/counit for $F\adjoint G$ and similar for $\varepsilon',\eta'$.
\end{definition}
We start by showing (a) implies (b). For this, we want to show $K\varepsilon_d=\varepsilon'_{Kd}$ for any $d\in\mc D$. We will show that
\[(K\varepsilon_d)^\sharp\stackrel?=(\varepsilon'_{Kd})^\sharp=\id_{G'Kd},\]
where we are transposing through $F'\adjoint G'$. On the other hand, pushing through the sharp on the left-hand side, we note
\[(K\varepsilon_d)^\sharp=G'(K\varepsilon_d)\circ\eta'_{G'Kd}=G'K\varepsilon_d\circ\eta'_{HGd}\stackrel*=HG\varepsilon_d\circ H\eta_{Gd}=H(G\varepsilon_d\circ\eta_{Gd}),\]
which is what we want after applying the triangle inequality and using the naturality of $H$; notably, we used $H\eta=\eta'H$ in $\stackrel*=$.

We now show (b) implies (c). Suppose $K\varepsilon=\varepsilon'K$, and we want our rectangle to commute. We simply diagram-chase in $\mathrm{Set}$: pick up some $f:Fc\to d$. Along the top, we track the following.
% https://q.uiver.app/?q=WzAsNSxbMCwwLCJmIl0sWzEsMCwiR2ZcXGNpcmNcXGV0YV9jIl0sWzEsMSwiSChHZlxcY2lyY1xcZXRhX2MpIl0sWzEsMiwiSChHZlxcY2lyY1xcZXRhX2MpIl0sWzAsMiwiXFx2YXJlcHNpbG9uX3tLZH0nXFxjaXJjIEYnSChHZlxcY2lyY1xcZXRhX2MpIl0sWzAsMV0sWzEsMl0sWzIsM10sWzMsNF1d
\[\begin{tikzcd}
	f & {Gf\circ\eta_c} \\
	& {H(Gf\circ\eta_c)} \\
	{\varepsilon_{Kd}'\circ F'H(Gf\circ\eta_c)} & {H(Gf\circ\eta_c)}
	\arrow[from=1-1, to=1-2]
	\arrow[from=1-2, to=2-2]
	\arrow[from=2-2, to=3-2]
	\arrow[from=3-2, to=3-1]
\end{tikzcd}\]
So we would like 
\[Kf\stackrel?=\varepsilon_{Kd}'\circ F'H(Gf\circ\eta_c).\]
Well, we can compute
\begin{align*}
	\varepsilon_{Kd}'\circ F'H(Gf\circ\eta_c) &= K\varepsilon_{d}\circ KF(Gf\circ\eta_c) \\
	&= K(\varepsilon_{d}\circ Gf)\circ KF\eta_c \\
	&= K(f\circ\varepsilon_{Fc})\circ KF\eta_c,
\end{align*}
where in the last equality we used the naturality of $\varepsilon$ as follows.
% https://q.uiver.app/?q=WzAsNCxbMCwwLCJGR0ZjIl0sWzEsMCwiRkdkIl0sWzEsMSwiZCJdLFswLDEsIkZjIl0sWzMsMiwiZiIsMl0sWzAsMSwiRkdmIl0sWzEsMiwiXFx2YXJlcHNpbG9uX2QiXSxbMCwzLCJcXHZhcmVwc2lsb25fe0ZjfSIsMl1d
\[\begin{tikzcd}
	FGFc & FGd \\
	Fc & d
	\arrow["f"', from=2-1, to=2-2]
	\arrow["FGf", from=1-1, to=1-2]
	\arrow["{\varepsilon_d}", from=1-2, to=2-2]
	\arrow["{\varepsilon_{Fc}}"', from=1-1, to=2-1]
\end{tikzcd}\]
Continuing to rearrange, we see that we have
\[Kf\circ K(\varepsilon_{Fc}\circ F\eta_c)=Kf,\]
where we have used the triangle equalities.

\end{document}